CollatzFunction/Halt/Search0.lean
@@ -8,14 +8,14 @@ open Lean Meta Elab Tactic Std Term TmState
 
 
 -- left
-theorem recD (k : ℕ): ∀ (i : ℕ) (l r : List Γ),
-nth_cfg i = some ⟨D, ⟨Γ.one,
+theorem recD (k : ℕ): ∀ (i : ℕ) (l r : List Γ) (init_cfg: Cfg),
+nth_cfg init_cfg i = some ⟨D, ⟨Γ.one,
   Turing.ListBlank.mk (List.replicate k Γ.one ++ List.cons Γ.zero l),
   Turing.ListBlank.mk r⟩⟩ →
-nth_cfg (i + k + 1) = some ⟨D, ⟨Γ.zero,
+nth_cfg init_cfg (i + k + 1) = some ⟨D, ⟨Γ.zero,
   Turing.ListBlank.mk l,
   Turing.ListBlank.mk (List.replicate (k+1) Γ.one ++ r)⟩⟩ := by
-induction k with intros i l r h
+induction k with intros i l r init_cfg h
 | zero => simp [nth_cfg, h, step, machine, Turing.Tape.write, Turing.Tape.move]
 | succ k induction_step =>
             specialize induction_step (i+1) l (List.cons Γ.one r)
@@ -24,14 +24,14 @@ induction k with intros i l r h
             . simp [List.replicate_succ']
             . simp! [nth_cfg, h, step, machine, Turing.Tape.write, Turing.Tape.move]
 
-theorem recJ (k : ℕ): ∀ (i : ℕ) (l r : List Γ),
-nth_cfg i = some ⟨J, ⟨Γ.one,
+theorem recJ (k : ℕ): ∀ (i : ℕ) (l r : List Γ) (init_cfg),
+nth_cfg init_cfg i = some ⟨J, ⟨Γ.one,
   Turing.ListBlank.mk (List.replicate k Γ.one ++ List.cons Γ.zero l),
   Turing.ListBlank.mk r⟩⟩ →
-nth_cfg (i + k + 1) = some ⟨J, ⟨Γ.zero,
+nth_cfg init_cfg (i + k + 1) = some ⟨J, ⟨Γ.zero,
   Turing.ListBlank.mk l,
   Turing.ListBlank.mk (List.replicate (k+1) Γ.one ++ r)⟩⟩ := by
-induction k with intros i l r h
+induction k with intros i l r init_cfg h
 | zero => simp [nth_cfg, h, step, machine, Turing.Tape.write, Turing.Tape.move]
 | succ k induction_step =>
             specialize induction_step (i+1) l (List.cons Γ.one r)
@@ -42,14 +42,14 @@ induction k with intros i l r h
 
 
 --right
-theorem recB (k : ℕ): ∀ (i : ℕ) (l r : List Γ),
-nth_cfg i = some ⟨B, ⟨Γ.one,
+theorem recB (k : ℕ): ∀ (i : ℕ) (l r : List Γ) (init_cfg),
+nth_cfg init_cfg i = some ⟨B, ⟨Γ.one,
   Turing.ListBlank.mk l,
   Turing.ListBlank.mk (List.replicate k Γ.one ++ List.cons Γ.zero r) ⟩⟩ →
-nth_cfg (i + k + 1) = some ⟨B, ⟨Γ.zero,
+nth_cfg init_cfg (i + k + 1) = some ⟨B, ⟨Γ.zero,
   Turing.ListBlank.mk (List.replicate (k+1) Γ.one ++ l),
   Turing.ListBlank.mk r⟩⟩ := by
-induction k with intros i l r h
+induction k with intros i l r init_cfg h
 | zero => simp [nth_cfg, h, step, machine, Turing.Tape.write, Turing.Tape.move]
 | succ k induction_step =>
             specialize induction_step (i+1) (List.cons Γ.one l) r
@@ -58,14 +58,14 @@ induction k with intros i l r h
             . simp [List.replicate_succ']
             . simp! [nth_cfg, h, step, machine, Turing.Tape.write, Turing.Tape.move]
 
-theorem recH (k : ℕ): ∀ (i : ℕ) (l r : List Γ),
-nth_cfg i = some ⟨H, ⟨Γ.one,
+theorem recH (k : ℕ): ∀ (i : ℕ) (l r : List Γ) (init_cfg: Cfg),
+nth_cfg init_cfg i = some ⟨H, ⟨Γ.one,
   Turing.ListBlank.mk l,
   Turing.ListBlank.mk (List.replicate k Γ.one ++ List.cons Γ.zero r) ⟩⟩ →
-nth_cfg (i + k + 1) = some ⟨H, ⟨Γ.zero,
+nth_cfg init_cfg (i + k + 1) = some ⟨H, ⟨Γ.zero,
   Turing.ListBlank.mk (List.replicate (k+1) Γ.one ++ l),
   Turing.ListBlank.mk r⟩⟩ := by
-induction k with intros i l r h
+induction k with intros i l r init_cfg h
 | zero => simp [nth_cfg, h, step, machine, Turing.Tape.write, Turing.Tape.move]
 | succ k induction_step =>
             specialize induction_step (i+1) (List.cons Γ.one l) r
