CollatzFunction/NonHalt/BStep.lean
@@ -5,12 +5,12 @@ namespace NonHalt
 
 open Lean Meta Elab Tactic Std Term TmState Γ
 
-lemma B_step (l r: List Γ) (n i: ℕ)
-(h : nth_cfg i =  ⟨B, ⟨one,
+lemma B_step (l r: List Γ) (n i: ℕ) (init_cfg: Cfg)
+(h : nth_cfg init_cfg i =  ⟨B, ⟨one,
   Turing.ListBlank.mk (List.cons zero l),
   Turing.ListBlank.mk (List.replicate (2+n) one ++ zero :: r)⟩⟩)
 :
-nth_cfg (9 + i + n * 2) =  ⟨B, ⟨one,
+nth_cfg init_cfg (9 + i + n * 2) =  ⟨B, ⟨one,
   Turing.ListBlank.mk (zero :: one :: l),
   Turing.ListBlank.mk (List.replicate n one ++ zero :: one :: r)⟩⟩
 := by
