CollatzFunction/NonHalt/Search1.lean
@@ -7,17 +7,17 @@ namespace NonHalt
 open Lean Meta Elab Tactic Std Term TmState
 
 --right
-theorem recF (k : ℕ): ∀ (i : ℕ) (l r : List Γ) (γ : Γ),
-nth_cfg i =  ⟨F, ⟨Γ.zero,
+theorem recF (k : ℕ): ∀ (i : ℕ) (l r : List Γ) (init_cfg : Cfg) (γ : Γ),
+nth_cfg init_cfg i =  ⟨F, ⟨Γ.zero,
   Turing.ListBlank.mk l,
   Turing.ListBlank.mk (List.replicate k Γ.zero ++ List.cons γ r) ⟩⟩ →
-nth_cfg (i + k + 1) =  ⟨F, ⟨γ,
+nth_cfg init_cfg (i + k + 1) =  ⟨F, ⟨γ,
   Turing.ListBlank.mk (List.replicate (k+1) Γ.zero ++ l),
   Turing.ListBlank.mk r⟩⟩ := by
-induction k with intros i l r γ h
+induction k with intros i l r init_cfg γ h
 | zero => simp [nth_cfg, h, step, machine, Turing.Tape.write, Turing.Tape.move]
 | succ k induction_step =>
-            specialize induction_step (i+1) (List.cons Γ.zero l) r γ
+            specialize induction_step (i+1) (List.cons Γ.zero l) r init_cfg γ
             have g : i + (k+1) +1 = i + 1 + k + 1 := by omega
             rw [g, induction_step]
             . simp [List.replicate_succ']
