CollatzFunction/NonHalt/Transition.lean
@@ -5,12 +5,12 @@ namespace NonHalt
 
 open Lean Meta Elab Tactic Std Term TmState Γ
 
-theorem lemma_G_to_H (r: List Γ)(r1: ℕ)(i : ℕ)(l: List Γ)
+theorem lemma_G_to_H (r: List Γ)(r1: ℕ)(i : ℕ)(l: List Γ)(init_cfg: Cfg)
 (h :
-nth_cfg i =  ⟨G, ⟨Γ.one,
+nth_cfg init_cfg i =  ⟨G, ⟨Γ.one,
   Turing.ListBlank.mk l,
   Turing.ListBlank.mk (List.replicate r1 Γ.one ++ List.cons Γ.zero r)⟩⟩) :
-nth_cfg (i+r1+1) =  ⟨H, ⟨Γ.zero,
+nth_cfg init_cfg (i+r1+1) =  ⟨H, ⟨Γ.zero,
   Turing.ListBlank.mk (List.replicate r1 Γ.one ++ List.cons Γ.zero l),
   Turing.ListBlank.mk r⟩⟩
 := by
@@ -22,12 +22,12 @@ cases r1 with
              ring_nf at *
              simp [h]
 
-theorem lemma_H_to_J (r: List Γ)(r1: ℕ)(i : ℕ)(l: List Γ)
+theorem lemma_H_to_J (r: List Γ)(r1: ℕ)(i : ℕ)(l: List Γ)(init_cfg: Cfg)
 (h :
-nth_cfg i =  ⟨H, ⟨Γ.zero,
+nth_cfg init_cfg i =  ⟨H, ⟨Γ.zero,
   Turing.ListBlank.mk (List.replicate r1 Γ.one ++ List.cons Γ.zero r),
   Turing.ListBlank.mk l⟩⟩) :
-nth_cfg (i+r1+1) =  ⟨J, ⟨Γ.zero,
+nth_cfg init_cfg (i+r1+1) =  ⟨J, ⟨Γ.zero,
   Turing.ListBlank.mk r,
   Turing.ListBlank.mk (List.replicate r1 Γ.one ++ List.cons Γ.one l)⟩⟩
 := by
